src/propositional_logic/syntactics.lean
@@ -1,7 +1,154 @@
 import propositional_logic.lanugage
-
+import data.set
 open formula
 
+@[derive [has_mem Formula, has_union, has_subset]]
+def Axioms := set Formula
+
+inductive deduction_consequence (ax : Axioms) (T : Theory) : Formula → Prop
+| is_theory : ∀ {φ : Formula}, φ ∈ T → deduction_consequence φ
+| is_axiom : ∀ {φ : Formula}, φ ∈ ax → deduction_consequence φ
+| is_modus_ponens : ∀ {φ ψ : Formula}, deduction_consequence φ → deduction_consequence (φ →ᶠ ψ) → deduction_consequence ψ
+
+def P1 : Axioms :=
+{ ζ : Formula | ∃ φ ψ   : Formula, ζ = φ →ᶠ (ψ →ᶠ φ)}
+def P2 : Axioms :=
+{ ζ : Formula | ∃ φ ψ ξ : Formula, ζ = (φ →ᶠ (ψ →ᶠ ξ)) →ᶠ ((φ →ᶠ ψ) →ᶠ (φ →ᶠ ξ))}
+def P3 : Axioms :=
+{ ζ : Formula | ∃ φ ψ   : Formula, ζ = (¬ᶠφ →ᶠ ¬ᶠψ) →ᶠ (ψ →ᶠ φ) }
+
+def classical_axioms : Axioms := 
+P1 ∪ P2 ∪ P3
+
+namespace classical_axioms
+
+variables {φ ψ ξ : Formula}
+
+lemma p1_subset_classical_axioms : P1 ⊆ classical_axioms :=
+set.subset.trans (set.subset_union_left _ P2) (set.subset_union_left _ P3)
+
+lemma p2_subset_classical_axioms : P2 ⊆ classical_axioms :=
+set.subset.trans (set.subset_union_right P1 _) (set.subset_union_left _ P3)
+
+lemma p3_subset_classical_axioms : P3 ⊆ classical_axioms :=
+set.subset_union_right _ P3
+
+lemma in_P1 : φ →ᶠ (ψ →ᶠ φ) ∈ P1 := ⟨φ, ψ, rfl⟩
+
+lemma in_P2 : (φ →ᶠ (ψ →ᶠ ξ)) →ᶠ ((φ →ᶠ ψ) →ᶠ (φ →ᶠ ξ)) ∈ P2 := ⟨φ, ψ, ξ, rfl⟩
+
+lemma in_P3 : (¬ᶠφ →ᶠ ¬ᶠψ) →ᶠ (ψ →ᶠ φ) ∈ P3 := ⟨φ, ψ, rfl⟩
+
+end classical_axioms
+
+def consequence : Theory → Formula → Prop :=
+deduction_consequence classical_axioms
+
 namespace syntactics
+
+open classical_axioms
+
+variables {T S : Theory} (φ ψ ξ : Formula)
+
+infix ` ⊢ `:50 := consequence
+
+lemma is_theory : φ ∈ T → consequence T φ := 
+λ _, deduction_consequence.is_theory ‹_›
+
+lemma is_axiom : φ ∈ classical_axioms → consequence T φ := 
+λ _, deduction_consequence.is_axiom ‹_›
+
+lemma is_modes_ponens : consequence T φ → consequence T (φ →ᶠ ψ) → consequence T ψ := 
+λ _  _, deduction_consequence.is_modus_ponens ‹_› ‹_›
+
+lemma is_P1 : T ⊢ φ →ᶠ (ψ →ᶠ φ) := is_axiom _ (p1_subset_classical_axioms in_P1)
+
+lemma is_P2 : T ⊢ (φ →ᶠ (ψ →ᶠ ξ)) →ᶠ ((φ →ᶠ ψ) →ᶠ (φ →ᶠ ξ)) :=
+is_axiom _ (p2_subset_classical_axioms in_P2)
+
+lemma is_P3 : T ⊢ (¬ᶠφ →ᶠ ¬ᶠψ) →ᶠ (ψ →ᶠ φ) :=
+is_axiom _ (p3_subset_classical_axioms in_P3)
+
+variables {φ ψ ξ}
+
+lemma consequence_mem (h : φ ∈ T) : T ⊢ φ := deduction_consequence.is_theory ‹_›
+
+lemma consequence_self : {φ} ⊢ φ := consequence_mem (set.mem_singleton _)
+
+lemma consequence_cut (h : ∀ ψ ∈ S, T ⊢ ψ) (hS : S ⊢ φ) : T ⊢ φ :=
+begin
+  induction hS with ψ hψS ψ hψax α β hαS hαβS hαT hαβT, 
+  { exact h ψ hψS },
+  { exact is_axiom _ ‹_› },
+  { exact is_modes_ponens _ _ ‹_› ‹_› }
+end
+
+lemma consequence_trans (h : S ⊆ T) (hS : S ⊢ φ) : T ⊢ φ :=
+consequence_cut (λ ψ _, consequence_mem (h ‹_›)) hS
+
+def is_true (φ : Formula) : Prop := ∅ ⊢ φ
+
+prefix ` ⊢ₜ `:40 := is_true
+
+lemma is_true_def : ⊢ₜ φ ↔ ∅ ⊢ φ := iff.rfl
+
+lemma consequence_of_is_true : ⊢ₜ φ → T ⊢ φ := 
+consequence_trans (set.empty_subset _)
+
+
+section deduction_theorem
+
+lemma is_true_self_to_self : ⊢ₜ φ →ᶠ φ  :=
+begin
+  apply is_modes_ponens (φ →ᶠ (φ →ᶠ φ)) _ (is_P1 _ _),
+  exact is_modes_ponens (φ →ᶠ ((φ →ᶠ φ) →ᶠ φ)) _ (is_P1 _ _) (is_P2 _ _ _),
+end
+
+lemma consequence_self_to_self : T ⊢ φ →ᶠ φ := 
+consequence_of_is_true is_true_self_to_self
+
+lemma consequence_union_singleton_of_consequence_to (h : T ⊢ φ →ᶠ ψ) : T ∪ {φ} ⊢ ψ :=
+begin
+  apply is_modes_ponens φ _,
+  {
+    apply is_theory,
+    simp,
+  },
+  {
+    refine consequence_trans _ h,
+    simp,
+  }
+end
+
+lemma consequence_to_of_consequence_union_singleton (h : T ∪ {φ} ⊢ ψ) : (T ⊢ φ →ᶠ ψ) :=
+begin
+  induction h with ξ hξTφ ξ hξax α β hαTφ hαβTφ hαT hαβT,
+  {
+    rw set.mem_union at hξTφ,
+    cases hξTφ,
+    {
+      exact is_modes_ponens _ _ (is_theory _ ‹_›) (is_P1 _ _)
+    },
+    {
+      rw set.mem_singleton_iff at hξTφ,
+      rw hξTφ,
+      exact consequence_self_to_self,
+    }
+  },
+  {
+    exact is_modes_ponens _ _ (is_axiom _ ‹_›) (is_P1 _ _)
+  },
+  {
+    apply is_modes_ponens _ _ hαT,
+    apply is_modes_ponens _ _ hαβT,
+    exact is_P2 _ _ _,
+  }
+end
+
+theorem deduction : (T ⊢ φ →ᶠ ψ) ↔ T ∪ {φ} ⊢ ψ :=
+⟨consequence_union_singleton_of_consequence_to, consequence_to_of_consequence_union_singleton⟩
+
+end deduction_theorem
+
 
 end syntactics
