src/propositional_logic/lanugage.lean
@@ -1,18 +1,54 @@
 import order
+import data.finset
+import data.pfun
 
-def index := ℕ
+open classical
+
+noncomputable theory
+
+@[derive [decidable_eq]]
+def var := ℕ
 
 inductive Formula : Type
-| Var : index → Formula
+| Var : var → Formula
 | To  : Formula → Formula → Formula
 | Not : Formula → Formula
+
+instance : inhabited Formula :=
+⟨Formula.Var (0 : ℕ)⟩
+
+instance : has_mem var Formula :=
+{mem := λ n φ, begin
+  induction φ with m φ ψ φmem ψmem φ φmem,
+  exact m = n,
+  exact φmem ∨ ψmem,
+  exact φmem,
+end}
+
+structure SubstitutionData := 
+(fn : pfun var Formula)
+(finite_dom : ∃ A : finset var, (A : set var) = fn.dom)
+
+
+class has_substitution (α : Type*) :=
+(substitute : α → SubstitutionData → α)
 
 namespace formula
 
 def Var := Formula.Var
 
 infix ` →ᶠ `:60 := Formula.To
-prefix `¬ᶠ `:40 := Formula.Not
+prefix `¬ᶠ `:70 := Formula.Not
+
+/-instance : has_substitution Formula :=
+⟨λ φ s,
+begin
+  induction φ with n,
+  refine @dite _ (n ∈ s.dom) (dec _) (λ _, pfun.fn s n ‹_›) (λ _, Var n),
+  exact Formula.To ‹_› ‹_›,
+  exact Formula.Not ‹_›,
+end⟩-/
+--⟨λ φ s, Formula.rec s (λ _ _, Formula.To) (λ _, Formula.Not) φ⟩
 
 end formula
 
